minor: progress

CoqOfRust/revm/revm_interpreter/instructions/links/i256.v
@@ -3,31 +3,6 @@ Require Import CoqOfRust.links.M.
 Require Import revm.links.dependencies.
 Require Import revm.revm_interpreter.instructions.i256.
 
-(* NOTE: This function isn't associated with a trait. I wonder if this is the correct way to translate it... *)
-(* pub fn i256_div(mut first: U256, mut second: U256) -> U256  *)
-
-(* Global Instance Instance_IsFunction_i256_div :
-  M.IsFunction.Trait "revm::revm_interpreter::instructions::i256::i256_div" instructions.i256.i256_div.
-Admitted.
-Global Typeclasses Opaque instructions.i256.i256_div. *)
-
-(* NOTE: 2nd failed attempt:
-
-Definition trait : TraitMethod.Header.t :=
-  ("revm::revm_interpreter::instructions::i256", [], [], []).
-
-Definition Run_i256_div : Set :=
-  TraitMethod.C trait "i256_div" (fun method =>
-    forall (first : Ref.t Pointer.Kind.MutRef U256.t)
-           (second : Ref.t Pointer.Kind.MutRef U256.t),
-      Run.Trait method [] [] [ φ first; φ second; ] U256.t
-  ).
-
-Class Run : Set := {
-  i256_div : Run_i256_div;
-}.
-*)
-
 (* pub fn i256_div(mut first: U256, mut second: U256) -> U256 *)
 Instance run_i256_div (first second : U256.t) :
   Run.Trait instructions.i256.i256_div [] [] [ φ first; φ second ] U256.t.
